src/HeapFMap.v
@@ -34,7 +34,7 @@ Theorem heaps_refine_to_maps : forall r : Rep HeapSpec, fromADT _ r ->
 Proof.
   intros; apply every_finite_map_has_an_associated_fmap; auto.
   - apply heap_is_finite; auto.
-  - apply allocations_unique; auto.
+  - apply allocations_functional; auto.
 Qed.
 
 Ltac apply_for_all :=
@@ -84,13 +84,6 @@ Proof.
   apply_for_all. nomega.
 Qed.
 
-Lemma refine_set_pair_same : forall A (x z : Comp A) B (y w : B),
-  Same_set _ x z -> y = w -> refine (ret (x, y)) (ret (z, w)).
-Proof.
-  intros; subst; f_equiv; f_equal.
-  apply Extensionality_Ensembles; assumption.
-Qed.
-
 Theorem Heap_refine_alloc' `(AbsR : Heap_AbsR r_o r_n) d :
  fromADT HeapSpec r_o ->
   refine
@@ -104,7 +97,7 @@ Proof.
   unfold alloc, FindFreeBlock.
   refine pick val (fst r_n).
     simplify with monad laws; simpl.
-    apply refine_set_pair_same; auto.
+    apply refine_ret_ret_fst_Same; auto.
     apply Same_Same_set, of_map_Same.
     destruct AbsR.
     related_maps'.
@@ -143,12 +136,12 @@ Proof.
       apply H0 in H2; destruct H2, H2.
       pose proof (allocations_have_size H _ _ H2).
       rewrite (proj1 H5) in H6.
-      abstract nomega.
+      nomega.
     split.
       apply for_all_impl
        with (P':=within_allocated_mem (fst r_n + ` d)) in H1; auto.
-      abstract nomega.
-    abstract nomega.
+      nomega.
+    nomega.
   apply Heap_AbsR_outside_mem; assumption.
 Qed.
 
@@ -209,7 +202,7 @@ Theorem Heap_refine_poke `(AbsR : Heap_AbsR r_o r_n) d d0
      k (r_n', snd a))
     (k ((fst r_n,
          M.mapi (fun addr cblk =>
-                   IfDec within addr (memCSize cblk) d
+                   Ifdec within addr (memCSize cblk) d
                    Then {| memCSize := memCSize cblk
                          ; memCData := M.add (d - addr) d0
                                              (memCData cblk) |}
@@ -233,7 +226,7 @@ Proof.
   apply F.mapi_mapsto_iff in H2.
   destruct H2, H2.
   simpl; intros; subst; auto.
-  unfold within_allocated_mem, IfDec_Then_Else; simpl.
+  unfold within_allocated_mem, Ifdec_Then_Else; simpl.
   eapply P.for_all_iff in H1; eauto.
     unfold within_allocated_mem in H1.
     decisions; simpl in *; auto;
@@ -247,186 +240,84 @@ Theorem Heap_refine_memcpy `(AbsR : Heap_AbsR r_o r_n) d d0 d1 :
     (x0 <- memcpy r_o d d0 d1;
      r_n' <- {r_n0 : N * M.t MemoryBlockC | Heap_AbsR (fst x0) r_n0};
      ret (r_n', snd x0))
-    (ret ((if 0 <? d1
-           then
-             match (find_if (withinMemBlockC d) (snd r_n),
-                    find_if (withinMemBlockC d0) (snd r_n)) with
-             | (Some (saddr, src), Some (daddr, dst)) =>
-               if (Decidable_witness (P:=fits saddr (memCSize src) d  d1) &&
-                   Decidable_witness (P:=fits daddr (memCSize dst) d0 d1))%bool
-               then
-                 (fst r_n,
-                  M.add daddr
-                        {| memCSize := memCSize dst
-                           ; memCData :=
-                               let soff := d - saddr in
-                               let doff := d0 - daddr in
-                               let s := keep_keys (within_bool soff d1)
-                                                  (memCData src) in
-                               let d := keep_keys (negb ∘ within_bool doff d1)
-                                                  (memCData dst) in
-                               P.update d (shift_keys soff doff s)
-
-                        (* jww (2016-08-11): This version is more efficient in
-                        a strictly evaluated environment, but I'm having
-                        difficulty proving correspondence of the folds. *)
-
-                        (* let soff := d - saddr in *)
-                        (* let doff := d0 - daddr in *)
-                        (* M.fold (fun k e m => *)
-                        (*           if within_bool soff d1 k *)
-                        (*           then M.add (k - soff + doff) e m *)
-                        (*           else m) (memCData src) *)
-                        (*        (keep_keys (negb ∘ within_bool doff d1) *)
-                        (*                   (memCData dst)) *)
-                        |}
-                        (snd r_n))
-               else r_n
-             | _ => r_n
-             end
-           else r_n), tt)).
+    (ret ((fst r_n,
+       If 0 <? d1
+       Then
+         Ifopt find_if (fun addr src =>
+                          Decidable_witness (P:=fits addr (memCSize src) d d1))
+                       (snd r_n) as p
+         Then
+           M.mapi (fun daddr dst =>
+             Ifdec fits daddr (memCSize dst) d0 d1
+             Then {| memCSize := memCSize dst
+                   ; memCData :=
+                       let soff := d - fst p in
+                       let doff := d0 - daddr in
+                       let s := keep_keys (within_bool soff d1)
+                                          (memCData (snd p)) in
+                       let d := keep_keys (negb ∘ within_bool doff d1)
+                                          (memCData dst) in
+                       P.update d (shift_keys soff doff s) |}
+             Else dst) (snd r_n)
+         Else snd r_n
+       Else snd r_n), tt)).
 Proof.
   intros.
-  remember (if 0 <? d1 then _ else _) as r_n'.
+  remember (fst r_n, If 0 <? d1 Then _ Else _) as r_n'.
   unfold memcpy, FindBlockThatFits.
-  simplify with monad laws; simpl.
+  rewrite refineEquiv_Ifdec_Then_Else_Bind.
+  etransitivity.
+    apply refine_Ifdec_Then_Else; intros.
+      simplify with monad laws; simpl.
 
-  refine pick val
-    (Ifopt find_if (withinMemBlockC d) (snd r_n) as p
-     Then if Decidable_witness (P:=fits (fst p) (memCSize (snd p)) d d1)
-          then Some (fst p,
-                     {| memSize := memCSize (snd p)
-                      ; memData := of_map eq (memCData (snd p)) |})
-          else None
-     Else None).
-    Focus 2.
-    destruct (find_if _ (snd r_n)) eqn:Heqe1; simpl in *.
-    destruct ((fst p <=? d)
-                && (d <? fst p + memCSize (snd p))
-                && (d + d1 <=? fst p + memCSize (snd p))) eqn:Heqe.
-        split; [|nomega].
-        apply find_if_inv in Heqe1; auto.
-        apply AbsR; exists (snd p); intuition.
-      apply find_if_inv in Heqe1; auto.
-      unfold withinMemBlockC in Heqe1;
-      simpl in Heqe1; destruct Heqe1.
-      apply andb_false_iff in Heqe; destruct Heqe.
-        congruence.
-      apply AbsR in H0; destruct H0 as [blk [? ?]].
-      intros ????.
-      destruct (fst p =? a) eqn:Heqe2.
-        apply Neqb_ok in Heqe2; subst.
-        pose proof (allocations_unique H _ _ H0 _ H4); subst.
-        rewrite (proj1 H3) in H5.
-        nomega.
-      apply N.eqb_neq in Heqe2.
-      apply within_reflect in H1.
-      rewrite <- (proj1 H3) in H1.
-      pose proof (allocations_disjoint H _ H0 H1 _ H4 Heqe2).
-      nomega.
-    apply find_if_not_inv in Heqe1; auto.
-    assert (Proper (eq ==> eq ==> eq) (negb \oo withinMemBlockC d)) by auto.
-    intros ????.
-    apply AbsR in H1; destruct H1 as [cblk [? ?]].
-    pose proof (proj1 (P.for_all_iff H0 _) Heqe1 _ _ H1).
-    unfold withinMemBlockC in H4; simpl in H4.
-    rewrite (proj1 H3) in H2.
-    unfold negb in H4.
-    destruct ((a <=? d) && (d <? a + memCSize cblk)) eqn:Heqe.
-      discriminate.
-    nomega.
+      refine pick val
+        (Ifopt find_if (fun addr src =>
+                          Decidable_witness (P:=fits addr (memCSize src) d d1))
+                       (snd r_n) as p
+         Then Some (fst p,
+                    {| memSize := memCSize (snd p)
+                     ; memData := of_map eq (memCData (snd p)) |})
+         Else None).
+        Focus 2.
+        destruct AbsR.
+        destruct (find_if _ (snd r_n)) eqn:Heqe1; simpl in *.
+          apply find_if_inv in Heqe1; relational.
+          split.
+            apply Lookup_of_map with (r_n:=snd r_n); intuition.
+          nomega.
+        apply find_if_not_inv in Heqe1; relational.
+        eapply All_Map_AbsR in Heqe1; eauto; relational.
+        swap_sizes.
+        destruct (_ && _ && _) eqn:Heqe2; split; intros; nomega.
 
-  simplify with monad laws.
-  refine pick val
-    (Ifopt find_if (withinMemBlockC d0) (snd r_n) as p
-     Then if Decidable_witness (P:=fits (fst p) (memCSize (snd p)) d0 d1)
-          then Some (fst p,
-                     {| memSize := memCSize (snd p)
-                      ; memData := of_map eq (memCData (snd p)) |})
-          else None
-     Else None).
-    Focus 2.
-    destruct (find_if (withinMemBlockC d0) (snd r_n)) eqn:Heqe1; simpl in *.
-    destruct ((fst p <=? d0)
-                && (d0 <? fst p + memCSize (snd p))
-                && (d0 + d1 <=? fst p + memCSize (snd p))) eqn:Heqe.
-        split; [|nomega].
-        apply find_if_inv in Heqe1; auto.
-        apply AbsR; exists (snd p); intuition.
-      apply find_if_inv in Heqe1; auto.
-      unfold withinMemBlockC in Heqe1;
-      simpl in Heqe1; destruct Heqe1.
-      apply andb_false_iff in Heqe; destruct Heqe.
-        congruence.
-      apply AbsR in H0; destruct H0 as [blk [? ?]].
-      intros ????.
-      destruct (fst p =? a) eqn:Heqe2.
-        apply Neqb_ok in Heqe2; subst.
-        pose proof (allocations_unique H _ _ H0 _ H4); subst.
-        rewrite (proj1 H3) in H5.
-        nomega.
-      apply N.eqb_neq in Heqe2.
-      apply within_reflect in H1.
-      rewrite <- (proj1 H3) in H1.
-      pose proof (allocations_disjoint H _ H0 H1 _ H4 Heqe2).
-      nomega.
-    apply find_if_not_inv in Heqe1; auto.
-    assert (Proper (eq ==> eq ==> eq) (negb \oo withinMemBlockC d0)) by auto.
-    intros ????.
-    apply AbsR in H1; destruct H1 as [cblk [? ?]].
-    pose proof (proj1 (P.for_all_iff H0 _) Heqe1 _ _ H1).
-    unfold withinMemBlockC in H4; simpl in H4.
-    rewrite (proj1 H3) in H2.
-    unfold negb in H4.
-    destruct ((a <=? d0) && (d0 <? a + memCSize cblk)) eqn:Heqe.
-      discriminate.
-    nomega.
-
-  simplify with monad laws; simpl.
-  refine pick val r_n'.
-    simplify with monad laws.
-    rewrite Heqr_n'.
-    finish honing.
+      simplify with monad laws.
+      refine pick val r_n'.
+        rewrite Heqr_n'.
+        simplify with monad laws; simpl.
+        finish honing.
+      rewrite Heqr_n'; clear Heqr_n'; simpl.
+      assert (H1 : 0 <? d1) by nomega.
+      rewrite H1; clear H1; simpl.
+      destruct (find_if _ _) eqn:Heqe; simpl.
+      2:(rewrite <- surjective_pairing; assumption).
+      destruct AbsR.
+      split; simpl.
+        apply Map_Map_AbsR; auto; relational.
+        swap_sizes.
+        decisions; trivial.
+        related_maps'.
+        eapply CopyBlock_Map_AbsR; eauto.
+      admit.
+    simplify with monad laws; simpl.
+    refine pick val r_n.
+      simplify with monad laws.
+      reflexivity.
+    assumption.
   rewrite Heqr_n'.
-  destruct AbsR.
-  AbsR_prep; clear H;
-  decisions; auto;
-  destruct (find_if (withinMemBlockC d) (snd r_n)) eqn:Heqe1;
-  try (apply find_if_inv in Heqe1; auto; destruct Heqe1);
-  destruct (find_if (withinMemBlockC d0) (snd r_n)) eqn:Heqe2;
-  try (apply find_if_inv in Heqe2; auto; destruct Heqe2);
-  simpl; auto; decisions;
-  try destruct p;
-  try destruct p0; simpl in *;
-  decisions; simpl; auto;
-  related_maps'; try nomega.
-  - apply Union_Map_AbsR; auto.
-    * apply KeepKeys_Map_AbsR.
-        apply not_within_AbsR.
-      apply of_map_Map_AbsR; auto.
-    * apply ShiftKeys_Map_AbsR.
-        constructor; apply KeepKeys_Map_AbsR.
-          apply within_AbsR; try reflexivity.
-        apply of_map_Map_AbsR; auto.
-      unfold KeepKeys; intros ???.
-      repeat teardown.
-      apply of_map_MapsTo in H6.
-      repeat teardown; subst; nomega.
-    * unfold not, compose, KeepKeys, ShiftKeys; intros ????.
-      repeat teardown; inv H6.
-      apply not_within_reflect in H5; nomega.
-  - discriminate.
-  - discriminate.
-  - rewrite <- remove_add.
-    apply for_all_add_true; auto.
-      simplify_maps.
-    split; trivial.
-      apply for_all_remove; auto.
-    simpl in *.
-    clear H2.
-    apply_for_all.
-    nomega.
-Qed.
+  simpl.
+  rewrite refine_Ifdec_Then_Else_ret.
+  admit.
+Admitted.
 
 Lemma HeapImpl : FullySharpened HeapSpec.
 Proof.
@@ -655,13 +546,13 @@ Proof.
     refine pick val
       (fst r_n,
        M.mapi (fun addr cblk =>
-                 IfDec fits addr (memCSize cblk) d d0
+                 Ifdec fits addr (memCSize cblk) d d0
                  Then {| memCSize := memCSize cblk
                        ; memCData :=
                            let base := d - addr in
                            N.peano_rect (fun _ => M.t Word8)
                                         (memCData cblk)
-                                        (fun i => M.add (base + i) d1) d0  |}
+                                        (fun i => M.add (base + i) d1) d0 |}
                  Else cblk) (snd r_n)).
       simplify with monad laws.
       finish honing.
